

Vypočtete derivaci

$$1) f(x) = 12 + x^2 \cdot 2^x$$

$$f'(x) = 0 + (x^2 \cdot 2^x)' = x^2 2^x \ln 2 + 2^x \cdot 2x = \\ = 2^x (x^2 \ln 2 + 2x)$$

$$2) f(x) = \sqrt{1-x^2}$$

$$f'(x) = \frac{1}{2} (1-x^2)^{-1/2} \cdot (-2x) = \frac{-x}{\sqrt{1-x^2}}$$

$$3) f(x) = \left( \sin^3\left(\frac{x}{4}\right) \right)' = 3 \cdot \sin^2\left(\frac{x}{4}\right) \cdot \frac{1}{4} \cdot \cos\left(\frac{x}{4}\right)$$

$$4) f(x) = \frac{1}{2}x - \frac{1}{2}\sin x \cos x$$

$$f'(x) = \frac{1}{2} - \frac{1}{2}(\sin^2 x + \cos^2 x) = \frac{1}{2}(\sin^2 x - \cos^2 x + 1) = \frac{1}{2}(\sin^2 x - \cos^2 x + (\sin^2 x + \cos^2 x)) = \frac{1}{2}(2\sin^2 x) = \sin^2 x$$

$$5) f(x) = x \cdot \ln \frac{x-1}{x+1}$$

$$f'(x) = \ln \frac{x-1}{x+1} + x \cdot \left( \ln \frac{x-1}{x+1} \right)' = \ln \frac{x-1}{x+1} + \frac{2x}{x^2-1}$$

$$\begin{aligned} \left( \ln \frac{x-1}{x+1} \right)' &= \frac{1}{\frac{x-1}{x+1}} \cdot \frac{(x+1) - (x-1)}{(x+1)^2} = \frac{x+1}{x-1} \cdot \frac{2}{(x+1)^2} = \\ &= \frac{2}{x^2-1} \end{aligned}$$

$$\begin{aligned}
 6) \lim_{x \rightarrow -2} \frac{\sqrt{6+x} - \sqrt{2-x}}{x+2} &= \lim_{x \rightarrow -2} \frac{6+x-2+x}{(\sqrt{6+x} + \sqrt{2-x})(x+2)} = \\
 &= \lim_{x \rightarrow -2} \frac{4+2x}{(\sqrt{6+x} + \sqrt{2-x})(x+2)} = \lim_{x \rightarrow -2} \frac{2}{\sqrt{6+x} + \sqrt{2-x}} = \\
 &= \frac{2}{2+2} = \frac{1}{2}
 \end{aligned}$$

$$7) \lim_{x \rightarrow 1} \frac{x^3 - 2x^2 + 2x - 1}{x^2 - 1}$$

Nejdříve upravitíme polynom;  $x^3 - 2x^2 + 2x - 1 = 2x(-x+1) + x^3 - 1 = (-2x)(x-1) + (x-1)(x^2+x+1) = (x-1)(x^2-x+1)$

$$\begin{aligned}
 \text{Potom tedy; } \lim_{x \rightarrow 1} \frac{(x-1)(x^2-x+1)}{(x-1)(x+1)} &= \lim_{x \rightarrow 1} \frac{x^2-x+1}{x+1} = \\
 &= \frac{1}{2}
 \end{aligned}$$